Fix a bug in LExpr's evaluator that generates wrong de bruijn index (#724)
This patch fixes a bug in LExpr.evalApp that invokes mkAbsOfArity which
generates wrong De Bruijn indices when the number of arguments of
Factory op is larger than 2.

`mkAbsOfArity` receives the number of arguments `n` and returns nested
abstractions with applications inside, where abs and app alternate. For
example, when the input was a Factory op f and first argument x and n =
2 (which means f is a ternary op), `mkAbsOfArity` returns:
```
\. (\. (f x) 0) 1    <--- index 1 doesn't make sense.
```

This bug is not easily observable, unless we have a free variable `x`
that has a function type, or there is a partial application of a Factory
app. However, it can still happen in the case like attached in
LExprEvalTests.lean:

```
-- '"Int.Add3 x y z"' is a ternary op registered to Factory, returning (x + y + z).

...

private def testStateFV : LState TestParams :=
  { testState with state := [[("f", (none, esM[~Int.Add3]))]] }

...

/-
This fails, instead it prints:
LExpr.app () (LExpr.app () (LExpr.app ()
  (LExpr.op () { name := "Int.Add3", metadata := () } none)
  (LExpr.const () Lambda.LConst.intConst 10))
  (LExpr.bvar () 1))                            <---- Dangling De Bruijn index appears
  (LExpr.const () Lambda.LConst.intConst 30)
-/
 #eval Lambda.LExpr.eval 100 test_ternary_fv.σ (esM[((((f : int → int → int → int) #10) #20) #30)])
```

This patch simply removes `mkAbsOfArity`, and invokes `eval n' (.app e1'
e2')` whenever there was reduction in the subexpressions of `.app`.


By submitting this pull request, I confirm that you can use, modify,
copy, and redistribute this contribution, under the terms of your
choice.

---------

Co-authored-by: Shilpi Goel <shigoel@gmail.com>

StrataTest/DL/Lambda/LExprEvalTests.lean
@@ -254,7 +254,21 @@ private def testBuiltIn : @Factory TestParams :=
       inputs := [("x", mty[int]), ("y", mty[int])],
       output := mty[int],
       body := some esM[((~Int.Add x) y)]
-    }]
+    },
+
+    { name := "Int.Add3",
+      inputs := [("x", mty[int]), ("y", mty[int]), ("z", mty[int])],
+      output := mty[int],
+      concreteEval := some (fun _e args => match args with
+                        | [e1, e2, e3] =>
+                          let e1i := LExpr.denoteInt e1
+                          let e2i := LExpr.denoteInt e2
+                          let e3i := LExpr.denoteInt e3
+                          match e1i, e2i, e3i with
+                          | some x, some y, some z =>
+                            .some (.intConst e1.metadata (x + y + z))
+                          | _, _, _ => .none
+                        | _ => .none) }]
 
 private def testState : LState TestParams :=
   let ans := LState.addFactory LState.init testBuiltIn
@@ -656,6 +670,34 @@ example: stuck test25 := by
     rename_i a a2 a3 he
     cases a3
     cases a2; unfold denoteInt at he; contradiction
+
+
+-- Ternary function applied through a state variable.
+
+private def testStateFV : LState TestParams :=
+  { testState with state := [[("f", (none, esM[~Int.Add3]))]] }
+
+def test_ternary_fv := TestCase.mk
+  testStateFV
+  esM[((((f : int → int → int → int) #10) #20) #30)]
+  esM[#60]
+
+/-- info: true -/
+#guard_msgs in
+#eval check test_ternary_fv
+
+example: steps_well test_ternary_fv := by
+  unfold steps_well Scopes.toEnv test_ternary_fv testStateFV
+  take_step; apply Step.reduce_1
+  · inhabited_metadata
+  · apply Step.reduce_1
+    · inhabited_metadata
+    · apply Step.reduce_1
+      · inhabited_metadata
+      · apply Step.expand_fvar; rfl
+  take_step; apply Step.eval_fn <;> try rfl
+  · inhabited_metadata
+  take_refl
 
 
 end EvalTest
